Locally Nameless: Automate most proofs. Add sums and a third flavour of unit elimination to STLC.

LocallyNameless/STLC.v
@@ -3,10 +3,11 @@ From FormalSystems Require Export LocallyNameless.LocallyNameless.
 (** * Types *)
 
 Inductive Ty : Type :=
-| TyFun  : Ty -> Ty -> Ty
-| TyUnit : Ty
+| TyFun   : Ty -> Ty -> Ty
+| TyUnit  : Ty
 | TyEmpty : Ty
-| TyProd : Ty -> Ty -> Ty.
+| TyProd  : Ty -> Ty -> Ty
+| TySum   : Ty -> Ty -> Ty.
 
 Fixpoint eq_dec_Ty (A B : Ty) : {A = B} + {A <> B}.
 Proof.
@@ -29,17 +30,21 @@ Defined.
 (** * Terms *)
 
 Inductive Tm : Type :=
-| fvar (a : Atom) : Tm
-| bvar  : nat -> Tm
-| abs   : Tm -> Tm
-| app   : Tm -> Tm -> Tm
-| unit  : Tm
-| elimUnit : Tm -> Tm -> Tm
-| elimUnit' : Tm -> Tm -> Tm
-| abort : Tm -> Tm
-| pair  : Tm -> Tm -> Tm
-| outl  : Tm -> Tm
-| outr  : Tm -> Tm.
+| fvar       : Atom -> Tm
+| bvar       : nat -> Tm
+| abs        : Tm -> Tm
+| app        : Tm -> Tm -> Tm
+| unit       : Tm
+| elimUnit   : Tm -> Tm -> Tm
+| elimUnit'  : Tm -> Tm -> Tm
+| elimUnit'' : Tm
+| abort      : Tm -> Tm
+| pair       : Tm -> Tm -> Tm
+| outl       : Tm -> Tm
+| outr       : Tm -> Tm
+| inl        : Tm -> Tm
+| inr        : Tm -> Tm
+| case       : Tm.
 
 Coercion fvar : Atom >-> Tm.
 Coercion bvar : nat >-> Tm.
@@ -47,8 +52,8 @@ Coercion bvar : nat >-> Tm.
 Fixpoint eq_dec_Tm (t u : Tm) : {t = u} + {t <> u}.
 Proof.
   decide equality.
-  - apply (eq_dec_Atom a a0).
-  - apply PeanoNat.Nat.eq_dec.
+  - exact (eq_dec_Atom a a0).
+  - exact (PeanoNat.Nat.eq_dec n n0).
 Defined.
 
 #[export, refine] Instance Decidable_eq_Tm :
@@ -69,52 +74,48 @@ Defined.
 #[export] Instance Open_Tm : Open nat Atom Tm :=
   fix open (t : Tm) (i : nat) (a : Atom) : Tm :=
     match t with
-    | fvar a     => fvar a
-    | bvar j     => if decide (i = j) then a else bvar j
-    | abs t'     => abs (open t' (S i) a)
-    | app t1 t2  => app (open t1 i a) (open t2 i a)
-    | unit       => unit
-    | elimUnit t1 t2 => elimUnit (open t1 i a) (open t2 (S i) a)
+    | fvar a          => fvar a
+    | bvar j          => if decide (i = j) then a else bvar j
+    | abs t'          => abs (open t' (S i) a)
+    | app t1 t2       => app (open t1 i a) (open t2 i a)
+    | unit            => unit
+    | elimUnit t1 t2  => elimUnit (open t1 i a) (open t2 (S i) a)
     | elimUnit' t1 t2 => elimUnit' (open t1 i a) (open t2 i a)
-    | abort t'   => abort (open t' i a)
-    | pair t1 t2 => pair (open t1 i a) (open t2 i a)
-    | outl t'    => outl (open t' i a)
-    | outr t'    => outr (open t' i a)
+    | elimUnit''      => elimUnit''
+    | abort t'        => abort (open t' i a)
+    | pair t1 t2      => pair (open t1 i a) (open t2 i a)
+    | outl t'         => outl (open t' i a)
+    | outr t'         => outr (open t' i a)
+    | inl t'          => inl (open t' i a)
+    | inr t'          => inr (open t' i a)
+    | case            => case
     end.
 
 #[export] Instance Close_Tm : Close nat Atom Tm :=
   fix close (t : Tm) (i : nat) (a : Atom) : Tm :=
     match t with
-    | fvar x     => if decide (a = x) then bvar i else fvar x
-    | bvar n     => bvar n
-    | abs t'     => abs (close t' (S i) a)
-    | app t1 t2  => app (close t1 i a) (close t2 i a)
-    | unit       => unit
-    | elimUnit t1 t2 => elimUnit (close t1 i a) (close t2 (S i) a)
+    | fvar x          => if decide (a = x) then bvar i else fvar x
+    | bvar n          => bvar n
+    | abs t'          => abs (close t' (S i) a)
+    | app t1 t2       => app (close t1 i a) (close t2 i a)
+    | unit            => unit
+    | elimUnit t1 t2  => elimUnit (close t1 i a) (close t2 (S i) a)
     | elimUnit' t1 t2 => elimUnit' (close t1 i a) (close t2 i a)
-    | abort t'   => abort (close t' i a)
-    | pair t1 t2 => pair (close t1 i a) (close t2 i a)
-    | outl t'    => outl (close t' i a)
-    | outr t'    => outr (close t' i a)
+    | elimUnit''      => elimUnit''
+    | abort t'        => abort (close t' i a)
+    | pair t1 t2      => pair (close t1 i a) (close t2 i a)
+    | outl t'         => outl (close t' i a)
+    | outr t'         => outr (close t' i a)
+    | inl t'          => inl (close t' i a)
+    | inr t'          => inr (close t' i a)
+    | case            => case
     end.
 
 #[export, refine] Instance OC_Tm :
   OC nat Atom Tm Open_Tm Close_Tm := {}.
 Proof.
   all: induction t; cbn; intros;
-  [
-    now decide_all                     |
-    now decide_all                     |
-    now rewrite IHt; congruence        |
-    now rewrite IHt1, IHt2             |
-    easy                               |
-    now rewrite IHt1, IHt2; congruence |
-    now rewrite IHt1, IHt2             |
-    now rewrite IHt                    |
-    now rewrite IHt1, IHt2             |
-    now rewrite IHt                    |
-    now rewrite IHt
-  ].
+    decide_all; rewrite 1?IHt, 1?IHt1, 1?IHt2; congruence.
 Qed.
 
 Lemma open_open :
@@ -123,38 +124,7 @@ Lemma open_open :
     t {{ i ~> a }} {{ j ~> b }} = t {{ i ~> a }} ->
       t {{ j ~> b }} = t.
 Proof.
-  induction t; cbn; intros * Hneq H.
-  - easy.
-  - now decide_all.
-  - inversion H.
-    f_equal.
-    now apply IHt in H1; [| lia].
-  - inversion H.
-    f_equal.
-    + now apply IHt1 in H1.
-    + now apply IHt2 in H2.
-  - easy.
-  - inversion H.
-    f_equal.
-    + now apply IHt1 in H1.
-    + now apply IHt2 in H2; [| lia].
-  - inversion H.
-    f_equal.
-    + now apply IHt1 in H1.
-    + now apply IHt2 in H2; [| lia].
-  - inversion H.
-    f_equal.
-    now apply IHt in H1.
-  - inversion H.
-    f_equal.
-    + now apply IHt1 in H1.
-    + now apply IHt2 in H2.
-  - inversion H.
-    f_equal.
-    now apply IHt in H1; [| lia].
-  - inversion H.
-    f_equal.
-    now apply IHt in H1; [| lia].
+  now induction t; cbn; intros i j u1 u2 Hij [=]; f_equal; [decide_all | eauto..].
 Qed.
 
 (** ** Locally nameless *)
@@ -168,10 +138,14 @@ match t with
 | unit       => []
 | elimUnit t1 t2 => fv t1 ++ fv t2
 | elimUnit' t1 t2 => fv t1 ++ fv t2
+| elimUnit'' => []
 | abort t'   => fv t'
 | pair t1 t2 => fv t1 ++ fv t2
 | outl t'    => fv t'
 | outr t'    => fv t'
+| inl t'     => fv t'
+| inr t'     => fv t'
+| case       => []
 end.
 
 #[export, refine] Instance LocallyNameless_Tm :
@@ -181,113 +155,21 @@ end.
 }.
 Proof.
   - unfold supports, Fresh'.
-    induction t; cbn.
+    induction t; cbn; only 1: rename a into b; intros a Ha;
+      try (now rewrite 1?IHt, 1?IHt1, 1?IHt2 by solve_fresh).
     + now firstorder decide_all.
-    + easy.
-    + intros a Hfresh.
-      f_equal.
-      now apply Fresh'_invariant, IHt.
-    + intros a Hfresh.
-      now rewrite IHt1, IHt2; only 2-3: solve_fresh.
-    + easy.
-    + intros a Hfresh.
-      f_equal.
-      * now rewrite IHt1 by solve_fresh.
-      * now rewrite close_invariant, IHt2 by solve_fresh.
-    + intros a Hfresh.
-      now rewrite IHt1, IHt2; only 2-3: solve_fresh.
-    + intros a Hfresh.
-      f_equal.
-      now apply Fresh'_invariant, IHt.
-    + intros a Hfresh.
-      now rewrite IHt1, IHt2; only 2-3: solve_fresh.
-    + intros a Hfresh.
-      f_equal.
-      now apply Fresh'_invariant, IHt.
-    + intros a Hfresh.
-      f_equal.
-      now apply Fresh'_invariant, IHt.
-  - unfold LocallyClosed.
-    induction t; cbn.
-    + exists 0.
-      intros _ _.
-      now exists (fresh []).
-    + exists (S n).
-      intros j Hij.
-      exists (fresh []).
-      now decide_all; lia.
-    + destruct IHt as [i IH].
-      exists i.
-      intros j Hij.
-      destruct (IH (S j) ltac:(lia)) as [a Ha].
-      exists a.
-      now rewrite Ha.
-    + destruct IHt1 as [i1 IH1], IHt2 as [i2 IH2].
-      exists (max i1 i2).
-      intros j Hle.
-      destruct
-        (IH1 (max i1 i2) ltac:(lia)) as [a1 Ha1],
-        (IH2 (max i1 i2) ltac:(lia)) as [a2 Ha2].
-      exists (fresh (fv t1 ++ fv t2 ++ [a1; a2])).
-      f_equal.
-      * rewrite (open_LocallyClosed _ i1); [easy | | now lia].
-        now rapply IH1.
-      * rewrite (open_LocallyClosed _ i2); [easy | | now lia].
-        now rapply IH2.
-    + now exists 0; intros _ _; exists (fresh []).
-    + destruct IHt1 as [i1 IH1], IHt2 as [i2 IH2].
-      exists (max i1 i2).
-      intros j Hle.
-      destruct
-        (IH1 (max i1 i2) ltac:(lia)) as [a1 Ha1],
-        (IH2 (max i1 i2) ltac:(lia)) as [a2 Ha2].
-      exists (fresh (fv t1 ++ fv t2 ++ [a1; a2])).
-      f_equal.
-      * rewrite (open_LocallyClosed _ i1); [easy | | now lia].
-        now rapply IH1.
-      * rewrite (open_LocallyClosed _ i2); [easy | | now lia].
-        now rapply IH2.
-    + destruct IHt1 as [i1 IH1], IHt2 as [i2 IH2].
-      exists (max i1 i2).
-      intros j Hle.
-      destruct
-        (IH1 (max i1 i2) ltac:(lia)) as [a1 Ha1],
-        (IH2 (max i1 i2) ltac:(lia)) as [a2 Ha2].
-      exists (fresh (fv t1 ++ fv t2 ++ [a1; a2])).
-      f_equal.
-      * rewrite (open_LocallyClosed _ i1); [easy | | now lia].
-        now rapply IH1.
-      * rewrite (open_LocallyClosed _ i2); [easy | | now lia].
-        now rapply IH2.
-    + destruct IHt as [i IH].
-      exists i; intros j Hij.
-      destruct (IH j Hij) as [a Ha].
-      exists a.
-      now rewrite Ha.
-    + destruct IHt1 as [i1 IH1], IHt2 as [i2 IH2].
-      exists (max i1 i2).
-      intros j Hle.
-      destruct
-        (IH1 (max i1 i2) ltac:(lia)) as [a1 Ha1],
-        (IH2 (max i1 i2) ltac:(lia)) as [a2 Ha2].
-      exists (fresh (fv t1 ++ fv t2 ++ [a1; a2])).
-      f_equal.
-      * rewrite (open_LocallyClosed _ i1); [easy | | now lia].
-        now rapply IH1.
-      * rewrite (open_LocallyClosed _ i2); [easy | | now lia].
-        now rapply IH2.
-    + destruct IHt as [i IH].
-      exists i.
-      intros j Hij.
-      destruct (IH j Hij) as [a Ha].
-      exists a.
-      now rewrite Ha.
-    + destruct IHt as [i IH].
-      exists i.
-      intros j Hij.
-      destruct (IH j Hij) as [a Ha].
-      exists a.
-      now rewrite Ha.
+    + now f_equal; rewrite close_invariant, IHt.
+    + rewrite IHt1 by solve_fresh; f_equal.
+      now rewrite close_invariant, IHt2 by solve_fresh.
+  - intros t.
+    setoid_rewrite LocallyClosed_forall.
+    induction t; cbn;
+      try (now exists 0);
+      try (now destruct IHt as [i IH]; exists i; intros j a Hij; rewrite IH; [| lia]);
+      try (now destruct IHt1 as [i1 IH1], IHt2 as [i2 IH2];
+        exists (max i1 i2); intros j a Hle; rewrite IH1, IH2; [| lia..]).
+    exists (S n); intros j a Hij.
+    now decide_all; lia.
 Defined.
 
 (** ** Characterization of local closure *)
@@ -318,6 +200,9 @@ Inductive LocallyClosed' : nat -> Tm -> Prop :=
     LocallyClosed' i t1 ->
     LocallyClosed' i t2 ->
     LocallyClosed' i (elimUnit' t1 t2)
+| LocallyClosed'_elimUnit'' :
+  forall (i : nat),
+    LocallyClosed' i elimUnit''
 | LocallyClosed'_abort :
   forall (i : nat) (t' : Tm),
     LocallyClosed' i t' -> LocallyClosed' i (abort t')
@@ -329,7 +214,17 @@ Inductive LocallyClosed' : nat -> Tm -> Prop :=
     LocallyClosed' i t' -> LocallyClosed' i (outl t')
 | LocallyClosed'_outr :
   forall (i : nat) (t' : Tm),
-    LocallyClosed' i t' -> LocallyClosed' i (outr t').
+    LocallyClosed' i t' -> LocallyClosed' i (outr t')
+| LocallyClosed'_inl :
+  forall (i : nat) (t' : Tm),
+    LocallyClosed' i t' -> LocallyClosed' i (inl t')
+| LocallyClosed'_inr :
+  forall (i : nat) (t' : Tm),
+    LocallyClosed' i t' -> LocallyClosed' i (inr t')
+| LocallyClosed'_case :
+  forall (i : nat),
+    LocallyClosed' i case.
+
 
 #[export] Hint Constructors LocallyClosed' : core.
 
@@ -337,110 +232,32 @@ Lemma LocallyClosed'_spec :
   forall (i : nat) (t : Tm),
     LocallyClosed' i t <-> LocallyClosed i t.
 Proof.
-  unfold LocallyClosed.
+  setoid_rewrite LocallyClosed_forall.
   split.
-  - induction 1; intros j Hij; cbn.
-    + now exists (fresh []).
-    + exists (fresh []).
-      now decide_all; lia.
-    + destruct (IHLocallyClosed' (S j) ltac:(lia)) as [a Ha].
-      now exists a; f_equal.
-    + destruct
-        (IHLocallyClosed'1 j Hij) as [a1 IH1],
-        (IHLocallyClosed'2 j Hij) as [a2 IH2].
-      exists (fresh (fv t1 ++ fv t2 ++ [a1; a2])).
-      f_equal.
-      * now rewrite open_invariant, IH1.
-      * now rewrite open_invariant, IH2.
-    + now exists (fresh []).
-    + destruct
-        (IHLocallyClosed'1 j Hij) as [a1 IH1],
-        (IHLocallyClosed'2 (S j) ltac:(lia)) as [a2 IH2].
-      exists (fresh (fv t1 ++ fv t2 ++ [a1; a2])).
-      f_equal.
-      * now rewrite open_invariant, IH1.
-      * now rewrite open_invariant, IH2.
-    + destruct
-        (IHLocallyClosed'1 j Hij) as [a1 IH1],
-        (IHLocallyClosed'2 j Hij) as [a2 IH2].
-      exists (fresh (fv t1 ++ fv t2 ++ [a1; a2])).
-      f_equal.
-      * now rewrite open_invariant, IH1.
-      * now rewrite open_invariant, IH2.
-    + destruct (IHLocallyClosed' j Hij) as [a Ha].
-      now exists a; f_equal.
-    + destruct
-        (IHLocallyClosed'1 j Hij) as [a1 IH1],
-        (IHLocallyClosed'2 j Hij) as [a2 IH2].
-      exists (fresh (fv t1 ++ fv t2 ++ [a1; a2])).
-      f_equal.
-      * now rewrite open_invariant, IH1.
-      * now rewrite open_invariant, IH2.
-    + destruct (IHLocallyClosed' j Hij) as [a Ha].
-      now exists a; f_equal.
-    + destruct (IHLocallyClosed' j Hij) as [a Ha].
-      now exists a; f_equal.
+  - induction 1; intros j a Hij; cbn; try (now f_equal; eauto).
+    + now decide_all; lia.
+    + now rewrite IHLocallyClosed'; [| lia].
+    + now rewrite IHLocallyClosed'1, IHLocallyClosed'2; [| lia..].
   - revert i.
-    induction t; cbn; intros i Hlc.
-    + now constructor.
-    + constructor.
-      destruct (PeanoNat.Nat.lt_ge_cases n i); [easy |].
-      destruct (Hlc _ H) as [a Ha].
+    induction t; cbn; intros i Hlc; constructor; try easy;
+    try match goal with
+    | IH : forall _, _ -> LocallyClosed' _ ?t  |- LocallyClosed' _ ?t =>
+      now apply IH; intros j a Hij; injection (Hlc j a Hij)
+    end.
+    + destruct (PeanoNat.Nat.lt_ge_cases n i); [easy |].
+      specialize (Hlc n (fresh []) H).
       now decide_all.
-    + constructor.
-      apply IHt; intros j Hle.
-      destruct j as [| j']; [now lia |].
-      destruct (Hlc j' ltac:(lia)) as [a [=] ].
-      now exists a.
-    + constructor.
-      * apply IHt1; intros j Hij.
-        destruct (Hlc j Hij) as [a Ha].
-        now exists a; congruence.
-      * apply IHt2; intros j Hij.
-        destruct (Hlc j Hij) as [a Ha].
-        now exists a; congruence.
-    + now constructor.
-    + constructor.
-      * apply IHt1; intros j Hij.
-        destruct (Hlc j Hij) as [a Ha].
-        now exists a; congruence.
-      * apply IHt2; intros j Hle.
-        destruct j as [| j']; [now lia |].
-        destruct (Hlc j' ltac:(lia)) as [a [=] ].
-        now exists a.
-    + constructor.
-      * apply IHt1; intros j Hij.
-        destruct (Hlc j Hij) as [a Ha].
-        now exists a; congruence.
-      * apply IHt2; intros j Hij.
-        destruct (Hlc j Hij) as [a Ha].
-        now exists a; congruence.
-    + constructor.
-      apply IHt; intros j Hij.
-      destruct (Hlc j Hij) as [a [=] ].
-      now exists a.
-    + constructor.
-      * apply IHt1; intros j Hij.
-        destruct (Hlc j Hij) as [a Ha].
-        now exists a; congruence.
-      * apply IHt2; intros j Hij.
-        destruct (Hlc j Hij) as [a Ha].
-        now exists a; congruence.
-    + constructor.
-      apply IHt; intros j Hij.
-      destruct (Hlc j Hij) as [a [=] ].
-      now exists a.
-    + constructor.
-      apply IHt; intros j Hij.
-      destruct (Hlc j Hij) as [a [=] ].
-      now exists a.
+    + apply IHt; intros [| j'] a Hle; [now lia |].
+      now injection (Hlc j' a ltac:(lia)).
+    + apply IHt2; intros [| j'] a Hle; [now lia |].
+      now injection (Hlc j' a ltac:(lia)).
 Qed.
 
 Lemma open_LocallyClosed' :
   forall (t : Tm) (i j : nat) (a : Atom),
     i <= j -> LocallyClosed' i t -> t {{ j ~> a }} = t.
 Proof.
-  intros.
+  intros t i j a Hij Hlc.
   apply open_LocallyClosed with j; [| now lia].
   now eapply LocallyClosed_le, LocallyClosed'_spec; eauto.
 Qed.
@@ -453,39 +270,14 @@ Lemma Fresh'_spec :
 Proof.
   split; [| now rapply supports_fv].
   unfold Fresh, Fresh'.
-  intros H.
-  induction t; cbn; intros.
-  - intros [-> |]; [| easy].
-    cbn in H.
-    now decide (x = x).
-  - easy.
+  induction t; cbn; intros [=]; rewrite ?in_app_iff;
+    try now firstorder congruence.
+  - now firstorder decide_all.
   - apply IHt.
-    cbn in H; inversion H; subst.
-    now rewrite close_close_eq.
-  - cbn in H; inversion H; subst.
-    rewrite H1, H2, in_app_iff.
-    now firstorder.
-  - easy.
-  - cbn in H; inversion H; subst.
-    rewrite H1, H2, in_app_iff.
-    intros []; firstorder.
+    now rewrite (close_invariant _ 0 1).
+  - intros []; [now apply IHt1; congruence |].
     apply IHt2; [| easy].
-    now rewrite <- H2, close_close_eq.
-  - cbn in H; inversion H; subst.
-    rewrite H1, H2, in_app_iff.
-    now firstorder.
-  - apply IHt.
-    cbn in H; inversion H; subst.
-    now rewrite close_close_eq.
-  - cbn in H; inversion H; subst.
-    rewrite H1, H2, in_app_iff.
-    now firstorder.
-  - apply IHt.
-    cbn in H; inversion H; subst.
-    now rewrite close_close_eq.
-  - apply IHt.
-    cbn in H; inversion H; subst.
-    now rewrite close_close_eq.
+    now rewrite (close_invariant _ 0 1).
 Qed.
 
 (** ** Substitution *)
@@ -499,10 +291,14 @@ match t with
 | unit       => unit
 | elimUnit t1 t2 => elimUnit (subst t1 x u) (subst t2 x u)
 | elimUnit' t1 t2 => elimUnit' (subst t1 x u) (subst t2 x u)
+| elimUnit'' => elimUnit''
 | abort t'   => abort (subst t' x u)
 | pair t1 t2 => pair (subst t1 x u) (subst t2 x u)
 | outl t'    => outl (subst t' x u)
 | outr t'    => outr (subst t' x u)
+| inl t'     => inl (subst t' x u)
+| inr t'     => inr (subst t' x u)
+| case       => case
 end.
 
 Notation "t [[ x := u ]]" := (subst t x u) (at level 68).
@@ -511,19 +307,8 @@ Lemma subst_fv :
   forall (t : Tm) (x : Atom) (u : Tm),
     x # fv t -> t [[ x := u ]] = t.
 Proof.
-  induction t; cbn; intros.
-  - decide_all.
-    now firstorder.
-  - easy.
-  - now rewrite IHt.
-  - now rewrite IHt1, IHt2; solve_fresh.
-  - easy.
-  - now rewrite IHt1, IHt2; solve_fresh.
-  - now rewrite IHt1, IHt2; solve_fresh.
-  - now rewrite IHt.
-  - now rewrite IHt1, IHt2; solve_fresh.
-  - now rewrite IHt.
-  - now rewrite IHt.
+  now induction t; cbn; intros;
+    [firstorder decide_all | rewrite 1?IHt, 1?IHt1, 1?IHt2 by solve_fresh..].
 Qed.
 
 (** ** Opening with a term *)
@@ -537,10 +322,14 @@ match t with
 | unit       => unit
 | elimUnit t1 t2 => elimUnit (open' t1 i u) (open' t2 (S i) u)
 | elimUnit' t1 t2 => elimUnit' (open' t1 i u) (open' t2 i u)
+    | elimUnit'' => elimUnit''
 | abort t'   => abort (open' t' i u)
 | pair t1 t2 => pair (open' t1 i u) (open' t2 i u)
 | outl t'    => outl (open' t' i u)
 | outr t'    => outr (open' t' i u)
+| inl t'     => inl (open' t' i u)
+| inr t'     => inr (open' t' i u)
+| case       => case
 end.
 
 Notation "t {[ i ~> u ]}" := (open' t i u) (at level 68).
@@ -557,18 +346,10 @@ Lemma open'_spec :
     x # fv t ->
       t {[ i ~> u ]} = t {{ i ~> x }} [[ x := u ]].
 Proof.
-  induction t; cbn; intros.
-  - now decide (x = a); subst; firstorder.
+  induction t; cbn; intros;
+    try now rewrite <- 1?IHt, 1?(IHt1 _ x), 1?(IHt2 _ x) by solve_fresh.
+  - now firstorder decide_all.
   - now decide_all.
-  - now rewrite <- IHt.
-  - now rewrite (IHt1 _ x), (IHt2 _ x); solve_fresh.
-  - easy.
-  - now rewrite (IHt1 _ x), (IHt2 _ x); solve_fresh.
-  - now rewrite (IHt1 _ x), (IHt2 _ x); solve_fresh.
-  - now rewrite <- IHt.
-  - now rewrite (IHt1 _ x), (IHt2 _ x); solve_fresh.
-  - now rewrite <- IHt.
-  - now rewrite <- IHt.
 Qed.
 
 Lemma open'_open' :
@@ -577,42 +358,7 @@ Lemma open'_open' :
     t {[ i ~> u1 ]} {[ j ~> u2 ]} = t {[ i ~> u1 ]} ->
       t {[ j ~> u2 ]} = t.
 Proof.
-  induction t; cbn; intros * Hneq H.
-  - easy.
-  - now decide_all.
-  - inversion H.
-    f_equal.
-    eapply IHt, H1.
-    now congruence.
-  - inversion H.
-    f_equal.
-    + now eapply IHt1, H1.
-    + now eapply IHt2, H2.
-  - easy.
-  - inversion H.
-    f_equal.
-    + now eapply IHt1, H1.
-    + now eapply IHt2, H2; lia.
-  - inversion H.
-    f_equal.
-    + now eapply IHt1, H1.
-    + now eapply IHt2, H2.
-  - inversion H.
-    f_equal.
-    eapply IHt, H1.
-    now congruence.
-  - inversion H.
-    f_equal.
-    + now eapply IHt1, H1.
-    + now eapply IHt2, H2.
-  - inversion H.
-    f_equal.
-    eapply IHt, H1.
-    now congruence.
-  - inversion H.
-    f_equal.
-    eapply IHt, H1.
-    now congruence.
+  now induction t; cbn; intros i j u1 u2 Hij [=]; f_equal; [decide_all | eauto..].
 Qed.
 
 (** ** Local closure *)
@@ -622,42 +368,52 @@ Inductive lc : Tm -> Prop :=
   forall x : Atom,
     lc x
 | lc_abs :
-  forall (t : Tm) (l : list Atom)
-    (Hcof : forall x : Atom, x # l -> lc (t {{ 0 ~> x }})),
-    lc (abs t)
+  forall (t' : Tm) (l : list Atom)
+    (Hlc' : forall x : Atom, x # l -> lc (t' {{ 0 ~> x }})),
+    lc (abs t')
 | lc_app :
-  forall t1 t2 : Tm,
-    lc t1 ->
-    lc t2 ->
+  forall (t1 t2 : Tm)
+    (Hlc1 : lc t1)
+    (Hlc2 : lc t2),
     lc (app t1 t2)
 | lc_unit : lc unit
 | lc_elimUnit :
   forall (t1 t2 : Tm) (l : list Atom)
     (Hlc1 : lc t1)
-    (Hcof : forall x : Atom, x # l -> lc (t2 {{ 0 ~> x }})),
+    (Hlc2 : forall x : Atom, x # l -> lc (t2 {{ 0 ~> x }})),
     lc (elimUnit t1 t2)
 | lc_elimUnit' :
   forall (t1 t2 : Tm)
     (Hlc1 : lc t1)
     (Hlc2 : lc t2),
     lc (elimUnit' t1 t2)
+| lc_elimUnit'' : lc elimUnit''
 | lc_abort :
-  forall t' : Tm,
-    lc t' ->
+  forall (t' : Tm)
+    (Hlc' : lc t'),
     lc (abort t')
 | lc_pair :
-  forall t1 t2 : Tm,
-    lc t1 ->
-    lc t2 ->
+  forall (t1 t2 : Tm)
+    (Hlc1 : lc t1)
+    (Hlc2 : lc t2),
     lc (pair t1 t2)
 | lc_outl :
-  forall t' : Tm,
-    lc t' ->
+  forall (t' : Tm)
+    (Hlc' : lc t'),
     lc (outl t')
 | lc_outr :
-  forall t' : Tm,
-    lc t' ->
-    lc (outr t').
+  forall (t' : Tm)
+    (Hlc' : lc t'),
+    lc (outr t')
+| lc_inl :
+  forall (t' : Tm)
+    (Hlc' : lc t'),
+    lc (inl t')
+| lc_inr :
+  forall (t' : Tm)
+    (Hlc' : lc t'),
+    lc (inr t')
+| lc_case : lc case.
 
 #[export] Hint Constructors lc : core.
 
@@ -665,48 +421,10 @@ Lemma LocallyClosed_lc :
   forall t : Tm,
     lc t -> LocallyClosed 0 t.
 Proof.
-  unfold LocallyClosed.
-  induction 1; cbn; intros j Hle.
-  - now exists x.
-  - destruct (H (fresh l) (fresh_spec l) (S j) ltac:(lia)) as [a Heq].
-    exists a.
-    f_equal.
-    now apply open_open in Heq.
-  - destruct (IHlc1 j Hle) as [a1 IH1].
-    destruct (IHlc2 j Hle) as [a2 IH2].
-    exists (fresh (fv t1 ++ fv t2 ++ [a1; a2])).
-    f_equal.
-    + now rewrite open_invariant, IH1.
-    + now rewrite open_invariant, IH2.
-  - now exists (fresh []).
-  - destruct (IHlc j Hle) as [a1 Ha1].
-    destruct (H0 (fresh l) (fresh_spec l) (S j) ltac:(lia)) as [a2 Ha2].
-    exists (fresh (fv t1 ++ fv t2 ++ [a1; a2])).
-    f_equal.
-    + now rewrite open_invariant, Ha1.
-    + apply open_open in Ha2; [| lia].
-      now rewrite open_invariant, Ha2.
-  - destruct (IHlc1 j Hle) as [a1 IH1].
-    destruct (IHlc2 j Hle) as [a2 IH2].
-    exists (fresh (fv t1 ++ fv t2 ++ [a1; a2])).
-    f_equal.
-    + now rewrite open_invariant, IH1.
-    + now rewrite open_invariant, IH2.
-  - destruct (IHlc j Hle) as [a Ha].
-    exists a.
-    now rewrite Ha.
-  - destruct (IHlc1 j Hle) as [a1 IH1].
-    destruct (IHlc2 j Hle) as [a2 IH2].
-    exists (fresh (fv t1 ++ fv t2 ++ [a1; a2])).
-    f_equal.
-    + now rewrite open_invariant, IH1.
-    + now rewrite open_invariant, IH2.
-  - destruct (IHlc j Hle) as [a Ha].
-    exists a.
-    now rewrite Ha.
-  - destruct (IHlc j Hle) as [a Ha].
-    exists a.
-    now rewrite Ha.
+  setoid_rewrite LocallyClosed_forall.
+  induction 1; cbn; intros j a Hle; f_equal; try now unshelve eauto.
+  - now eapply open_open, (H _ (fresh_spec l)); lia.
+  - now eapply open_open, (H0 _ (fresh_spec l)); lia.
 Qed.
 
 Lemma open_lc :
@@ -731,18 +449,8 @@ Lemma open_subst :
       =
     t [[ x := b ]] {{ i ~> if decide (a = x) then b else a }}.
 Proof.
-  induction t; cbn; intros.
-  - now decide_all.
-  - now decide_all.
-  - now rewrite IHt.
-  - now rewrite IHt1, IHt2.
-  - easy.
-  - now rewrite IHt1, IHt2.
-  - now rewrite IHt1, IHt2.
-  - now rewrite IHt.
-  - now rewrite IHt1, IHt2.
-  - now rewrite IHt.
-  - now rewrite IHt.
+  now induction t; cbn; intros;
+    [decide_all | decide_all | rewrite 1?IHt, 1?IHt1, 1?IHt2..].
 Qed.
 
 Lemma subst_open :
@@ -750,19 +458,10 @@ Lemma subst_open :
     a <> b -> lc u ->
     t [[ a := u ]] {{ i ~> b }} = t {{ i ~> b }} [[ a := u ]].
 Proof.
-  induction t; cbn; intros.
+  induction t; cbn; intros; [| | now rewrite 1?IHt, 1?IHt1, 1?IHt2..].
   - decide_all.
     now rewrite open_lc.
   - now decide_all.
-  - now rewrite IHt.
-  - now rewrite IHt1, IHt2.
-  - easy.
-  - now rewrite IHt1, IHt2.
-  - now rewrite IHt1, IHt2.
-  - now rewrite IHt.
-  - now rewrite IHt1, IHt2.
-  - now rewrite IHt.
-  - now rewrite IHt.
 Qed.
 
 Lemma lc_subst :
@@ -770,26 +469,14 @@ Lemma lc_subst :
     lc t -> lc u -> lc (t [[ x := u ]]).
 Proof.
   intros t x u Ht Hu; revert x u Hu.
-  induction Ht; cbn; intros.
+  induction Ht; cbn; intros; try now eauto.
   - now decide_all.
   - apply lc_abs with (x :: l).
-    intros y Hin.
-    rewrite subst_open; [| now firstorder | easy].
-    apply H; [| easy].
-    now firstorder.
-  - now constructor; [apply IHHt1 | apply IHHt2].
-  - now constructor.
-  - apply lc_elimUnit with (x :: l).
-    + now apply IHHt.
-    + intros y Hy.
-    rewrite subst_open; [| now firstorder | easy].
-    apply H; [| easy].
-    now firstorder.
-  - now constructor; [apply IHHt1 | apply IHHt2].
-  - now constructor; apply IHHt.
-  - now constructor; [apply IHHt1 | apply IHHt2].
-  - now constructor; apply IHHt.
-  - now constructor; apply IHHt.
+    intros y Hy.
+    now rewrite subst_open; firstorder.
+  - apply lc_elimUnit with (x :: l); [now apply IHHt |].
+    intros y Hy.
+    now rewrite subst_open; firstorder.
 Qed.
 
 Lemma open'_lc :
@@ -812,7 +499,7 @@ Proof.
   inversion 1; intros Hu.
   rewrite (open'_spec _ _ (fresh (l ++ fv t))) by solve_fresh.
   apply lc_subst; [| easy].
-  apply Hcof.
+  apply Hlc'.
   now solve_fresh.
 Qed.
 
@@ -820,8 +507,7 @@ Lemma lc_open'' :
   forall (t : Tm) (i : nat) (u : Tm),
     lc t -> lc (t {[ i ~> u ]}).
 Proof.
-  intros.
-  now rewrite open'_lc.
+  now intros; rewrite open'_lc.
 Qed.
 
 Lemma open'_subst :
@@ -831,19 +517,10 @@ Lemma open'_subst :
       =
     t [[ x := u2 ]] {[ i ~> u1 [[ x := u2 ]] ]}.
 Proof.
-  induction t; cbn; intros.
+  induction t; cbn; intros; [| | now rewrite 1?IHt, 1?IHt1, 1?IHt2..].
   - decide_all.
     now rewrite open'_lc.
   - now decide_all.
-  - now rewrite IHt.
-  - now rewrite IHt1, IHt2.
-  - easy.
-  - now rewrite IHt1, IHt2.
-  - now rewrite IHt1, IHt2.
-  - now rewrite IHt.
-  - now rewrite IHt1, IHt2.
-  - now rewrite IHt.
-  - now rewrite IHt.
 Qed.
 
 (** * Contexts *)
@@ -851,11 +528,12 @@ Qed.
 Definition Ctx : Type := list (Atom * Ty).
 
 Inductive WfCtx : Ctx -> Prop :=
-| WfCtx_nil  :
-  WfCtx []
+| WfCtx_nil  : WfCtx []
 | WfCtx_cons :
-    forall (Γ : Ctx) (x : Atom) (A : Ty),
-      WfCtx Γ -> x # map fst Γ -> WfCtx ((x, A) :: Γ).
+    forall (Γ : Ctx) (x : Atom) (A : Ty)
+      (Hwf : WfCtx Γ)
+      (Hdom : x # map fst Γ),
+      WfCtx ((x, A) :: Γ).
 
 #[export] Hint Constructors WfCtx : core.
 
@@ -865,10 +543,12 @@ Lemma WfCtx_app_cons :
 Proof.
   induction Γ2 as [| [y B] Γ2' IH]; cbn; inversion 1; [easy |].
   constructor.
-  - now apply IH in H2.
+  - now apply IH in Hwf.
   - unfold Fresh in *; rewrite map_app, !in_app_iff in *; cbn in *.
     now firstorder.
 Qed.
+
+#[export] Hint Resolve WfCtx_app_cons : core.
 
 (** * Binding variables in context *)
 
@@ -880,16 +560,14 @@ Lemma Binds_inv :
     WfCtx Γ -> Binds Γ x A -> Binds Γ x B -> A = B.
 Proof.
   induction 1; cbn; [easy |].
-  intros [ [= -> ->] |].
-  - intros [ [= ->] |]; [easy |].
-    contradiction H0.
+  intros [ [= -> ->] |] [ [= ->] |]; [easy | ..].
+  - contradiction Hdom.
     rewrite in_map_iff.
     now exists (x, B).
-  - intros [ [= -> ->] |].
-    + contradiction H0.
-      rewrite in_map_iff.
-      now exists (x, A).
-    + now apply IHWfCtx.
+  - contradiction Hdom.
+    rewrite in_map_iff.
+    now exists (x, A).
+  - now apply IHWfCtx.
 Qed.
 
 Lemma Binds_app_cons_inv :
@@ -901,8 +579,8 @@ Lemma Binds_app_cons_inv :
 Proof.
   induction Δ; cbn.
   - now firstorder congruence.
-  - inversion 1; subst; [now firstorder |].
-    apply IHΔ in H0.
+  - intros x y A B [ [= ->] | ]; [now firstorder |].
+    apply IHΔ in H.
     now firstorder.
 Qed.
 
@@ -915,66 +593,69 @@ Inductive Typing : Ctx -> Tm -> Ty -> Prop :=
     (HB : Binds Γ x A),
     Typing Γ x A
 | Typing_abs :
-  forall (Γ : Ctx) (t : Tm) (A B : Ty) (l : list Atom)
-    (Hcof : forall x : Atom, x # l -> Typing ((x, A) :: Γ) (t {{ 0 ~> x }}) B),
-    Typing Γ (abs t) (TyFun A B)
+  forall (Γ : Ctx) (t' : Tm) (A B : Ty) (l : list Atom)
+    (Ht' : forall x : Atom, x # l -> Typing ((x, A) :: Γ) (t' {{ 0 ~> x }}) B),
+    Typing Γ (abs t') (TyFun A B)
 | Typing_app :
-  forall (Γ : Ctx) (t1 t2 : Tm) (A B : Ty),
-    Typing Γ t1 (TyFun A B) ->
-    Typing Γ t2 A ->
+  forall (Γ : Ctx) (t1 t2 : Tm) (A B : Ty)
+    (Ht1 : Typing Γ t1 (TyFun A B))
+    (Ht2 : Typing Γ t2 A),
     Typing Γ (app t1 t2) B
 | Typing_unit :
-  forall (Γ : Ctx),
-    WfCtx Γ ->
+  forall (Γ : Ctx)
+    (Hwf : WfCtx Γ),
     Typing Γ unit TyUnit
 | Typing_elimUnit :
-  forall (Γ : Ctx) (t1 t2 : Tm) (A : Ty) (l : list Atom),
-    Typing Γ t1 TyUnit ->
-    forall (Hcof : forall x : Atom, x # l -> Typing ((x, TyUnit) :: Γ) (t2 {{ 0 ~> x }}) A),
+  forall (Γ : Ctx) (t1 t2 : Tm) (A : Ty) (l : list Atom)
+    (Ht1 : Typing Γ t1 TyUnit)
+    (Ht2 : forall x : Atom, x # l -> Typing ((x, TyUnit) :: Γ) (t2 {{ 0 ~> x }}) A),
     Typing Γ (elimUnit t1 t2) A
 | Typing_elimUnit' :
-  forall (Γ : Ctx) (t1 t2 : Tm) (A : Ty),
-    Typing Γ t1 TyUnit ->
-    Typing Γ t2 (TyFun TyUnit A) ->
+  forall (Γ : Ctx) (t1 t2 : Tm) (A : Ty)
+    (Ht1 : Typing Γ t1 TyUnit)
+    (Ht2 : Typing Γ t2 (TyFun TyUnit A)),
     Typing Γ (elimUnit' t1 t2) A
+| Typing_elimUnit'' :
+  forall (Γ : Ctx) (A : Ty)
+    (Hwf : WfCtx Γ),
+    Typing Γ elimUnit'' (TyFun (TyFun TyUnit A) (TyFun TyUnit A))
 | Typing_abort :
-  forall (Γ : Ctx) (t' : Tm) (A : Ty),
-    Typing Γ t' TyEmpty ->
+  forall (Γ : Ctx) (t' : Tm) (A : Ty)
+    (Ht' : Typing Γ t' TyEmpty),
     Typing Γ (abort t') A
 | Typing_pair :
-  forall (Γ : Ctx) (t1 t2 : Tm) (A B : Ty),
-    Typing Γ t1 A ->
-    Typing Γ t2 B ->
+  forall (Γ : Ctx) (t1 t2 : Tm) (A B : Ty)
+    (Ht1 : Typing Γ t1 A)
+    (Ht2 : Typing Γ t2 B),
     Typing Γ (pair t1 t2) (TyProd A B)
 | Typing_outl :
-  forall (Γ : Ctx) (t' : Tm) (A B : Ty),
-    Typing Γ t' (TyProd A B) ->
+  forall (Γ : Ctx) (t' : Tm) (A B : Ty)
+    (Ht' : Typing Γ t' (TyProd A B)),
     Typing Γ (outl t') A
 | Typing_outr :
-  forall (Γ : Ctx) (t' : Tm) (A B : Ty),
-    Typing Γ t' (TyProd A B) ->
-    Typing Γ (outr t') B.
+  forall (Γ : Ctx) (t' : Tm) (A B : Ty)
+    (Ht' : Typing Γ t' (TyProd A B)),
+    Typing Γ (outr t') B
+| Typing_inl :
+  forall (Γ : Ctx) (t' : Tm) (A B : Ty)
+    (Ht' : Typing Γ t' A),
+    Typing Γ (inl t') (TySum A B)
+| Typing_inr :
+  forall (Γ : Ctx) (t' : Tm) (A B : Ty)
+    (Ht' : Typing Γ t' B),
+    Typing Γ (inr t') (TySum A B)
+| Typing_case :
+  forall (Γ : Ctx) (A B C : Ty)
+    (Hwf : WfCtx Γ),
+    Typing Γ case (TyFun (TyFun A C) (TyFun (TyFun B C) (TyFun (TySum A B) C))).
 
-#[export] Hint Constructors Typing : Core.
+#[export] Hint Constructors Typing : core.
 
 Lemma lc_Typing :
   forall (Γ : Ctx) (t : Tm) (A : Ty),
     Typing Γ t A -> lc t.
 Proof.
-  induction 1.
-  - now constructor.
-  - apply lc_abs with l; intros x Hx.
-    now apply H.
-  - now constructor.
-  - now constructor.
-  - apply lc_elimUnit with l; [easy |].
-    intros x Hx.
-    now apply H0.
-  - now constructor.
-  - now constructor.
-  - now constructor.
-  - now constructor.
-  - now constructor.
+  now induction 1; eauto.
 Qed.
 
 Lemma WfCtx_Typing :
@@ -985,6 +666,8 @@ Proof.
   apply (WfCtx_app_cons _ [] (fresh l) A), H.
   now solve_fresh.
 Qed.
+
+#[export] Hint Resolve lc_Typing WfCtx_Typing : core.
 
 (** ** Weakening *)
 
@@ -997,43 +680,26 @@ Proof.
   intros * Ht.
   remember (Γ1 ++ Γ2) as G.
   revert Γ1 Γ2 Δ HeqG.
-  induction Ht; intros; subst.
+  induction Ht; intros; subst; try now unshelve eauto.
   - constructor; [easy |].
     unfold Binds in *.
     rewrite !in_app_iff; rewrite in_app_iff in HB.
     now firstorder.
   - apply Typing_abs with (l ++ map fst Γ1 ++ map fst Δ ++ map fst Γ2).
     intros x Hx.
-    red in Hx; rewrite !in_app_iff in Hx.
     rewrite app_comm_cons.
-    apply H; [now firstorder | easy |].
+    apply H; [now solve_fresh | easy |].
     cbn; constructor; [easy |].
-    red; rewrite !map_app, !in_app_iff.
-    now firstorder.
-  - apply Typing_app with A.
-    + now apply IHHt1.
-    + now apply IHHt2.
-  - now constructor.
-  - apply Typing_elimUnit with (l ++ map fst Γ1 ++ map fst Δ ++ map fst Γ2).
-    + now apply IHHt.
-    + intros x Hx.
-      red in Hx; rewrite !in_app_iff in Hx.
-      rewrite app_comm_cons.
-      apply H; [now firstorder | easy |].
-      cbn; constructor; [easy |].
-      red; rewrite !map_app, !in_app_iff.
-      now firstorder.
-  - constructor.
-    + now apply IHHt1.
-    + now apply IHHt2.
-  - now constructor; apply IHHt.
-  - constructor.
-    + now apply IHHt1.
-    + now apply IHHt2.
-  - apply Typing_outl with B.
-    now apply IHHt.
-  - apply Typing_outr with A.
-    now apply IHHt.
+    rewrite !map_app.
+    now solve_fresh.
+  - apply Typing_elimUnit with (l ++ map fst Γ1 ++ map fst Δ ++ map fst Γ2);
+      [now apply IHHt |].
+    intros x Hx.
+    rewrite app_comm_cons.
+    apply H; [now solve_fresh | easy |].
+    cbn; constructor; [easy |].
+    rewrite !map_app.
+    now solve_fresh.
 Qed.
 
 Lemma weakening :
@@ -1044,6 +710,8 @@ Lemma weakening :
 Proof.
   now intros; apply weakening_aux with (Γ1 := []); cbn.
 Qed.
+
+#[export] Hint Resolve weakening_aux weakening : core.
 
 (** ** Substitution *)
 
@@ -1056,44 +724,26 @@ Proof.
   intros * Ht Hu.
   remember (Δ ++ (x, A) :: Γ) as G.
   revert Δ x A Γ HeqG Hu.
-  induction Ht; cbn; intros; subst.
+  induction Ht; cbn; intros; subst; try now unshelve eauto.
   - apply WfCtx_app_cons in Hwf as Hwf'.
     decide (x0 = x); subst.
-    + replace A with A0.
-      * now apply weakening.
-      * symmetry.
-        eapply (Binds_inv _ _ _ _ Hwf HB).
-        red; rewrite in_app_iff; cbn.
-        now firstorder.
+    + replace A with A0; [now apply weakening |].
+      symmetry.
+      eapply (Binds_inv _ _ _ _ Hwf HB).
+      red; rewrite in_app_iff; cbn.
+      now firstorder.
     + apply Binds_app_cons_inv in HB as [ [-> ->] |]; [easy |].
       now constructor.
   - apply Typing_abs with (x :: l).
     intros y Hy.
     assert (x <> y /\ y # l) as [Hxy Hyl] by firstorder.
-    rewrite subst_open; [| now firstorder | now apply lc_Typing in Hu].
+    rewrite subst_open by eauto.
     now eapply (H y Hyl ((y, A) :: Δ)).
-  - econstructor.
-    + now eapply IHHt1.
-    + now eapply IHHt2.
-  - constructor.
-    now apply WfCtx_app_cons in H.
-  - apply Typing_elimUnit with (x :: l).
-    + now eapply IHHt.
-    + intros y Hy.
-      assert (x <> y /\ y # l) as [Hxy Hyl] by firstorder.
-      rewrite subst_open; [| now firstorder | now apply lc_Typing in Hu].
-      now eapply (H y Hyl ((y, TyUnit) :: Δ)).
-  - econstructor.
-    + now eapply IHHt1.
-    + now eapply IHHt2.
-  - now constructor; eapply IHHt.
-  - constructor.
-    + now eapply IHHt1.
-    + now eapply IHHt2.
-  - apply Typing_outl with B.
-    now eapply IHHt.
-  - apply Typing_outr with A.
-    now eapply IHHt.
+  - apply Typing_elimUnit with (x :: l); [now eapply IHHt |].
+    intros y Hy.
+    assert (x <> y /\ y # l) as [Hxy Hyl] by firstorder.
+    rewrite subst_open; [| now firstorder | now eauto].
+    now eapply (H y Hyl ((y, TyUnit) :: Δ)).
 Qed.
 
 Lemma Typing_subst :
@@ -1105,6 +755,8 @@ Proof.
   now intros; eapply Typing_subst_aux with (Δ := []) (A := A).
 Qed.
 
+#[export] Hint Resolve Typing_subst_aux Typing_subst : core.
+
 (** * Computation *)
 
 (** ** Values *)
@@ -1115,6 +767,7 @@ Inductive Value : Tm -> Prop :=
     lc (abs t) ->
     Value (abs t)
 | Value_unit : Value unit
+| Value_elimUnit'' : Value elimUnit''
 | Value_abort :
   forall t' : Tm,
     lc t' ->
@@ -1123,7 +776,25 @@ Inductive Value : Tm -> Prop :=
   forall t1 t2 : Tm,
     Value t1 ->
     Value t2 ->
-    Value (pair t1 t2).
+    Value (pair t1 t2)
+| Value_inl :
+  forall v : Tm,
+    Value v ->
+    Value (inl v)
+| Value_inr :
+  forall v : Tm,
+    Value v ->
+    Value (inr v)
+| Value_case : Value case
+| Value_case1 :
+  forall (t1 : Tm),
+    lc t1 ->
+    Value (app case t1)
+| Value_case2 :
+  forall (t1 t2 : Tm)
+    (Hlc1 : lc t1)
+    (Hlc2 : lc t2),
+    Value (app (app case t1) t2).
 
 #[export] Hint Constructors Value : core.
 
@@ -1134,57 +805,75 @@ Proof.
   now induction 1; eauto.
 Qed.
 
-(** *** Computation *)
+#[export] Hint Resolve lc_Value : core.
+
+(** * Computation *)
 
 (** ** Contraction *)
 
 Inductive Contraction : Tm -> Tm -> Prop :=
 | Contraction_Fun :
-  forall (t1 t2 : Tm),
-    lc (abs t1) ->
-    Value t2 ->
+  forall (t1 t2 : Tm)
+    (Hlc1 : lc (abs t1))
+    (Hv2 : Value t2),
     Contraction (app (abs t1) t2) (t1 {[ 0 ~> t2 ]})
 | Contraction_Unit :
   forall (t : Tm) (l : list Atom)
-    (Hcof : forall x : Atom, x # l -> lc (t {{0 ~> x}})),
+    (Hlc : forall x : Atom, x # l -> lc (t {{0 ~> x}})),
     Contraction (elimUnit unit t) (t {[ 0 ~> unit ]})
 | Contraction_Unit' :
-  forall (t : Tm),
-    lc t ->
+  forall (t : Tm)
+    (Hlc : lc t),
     Contraction (elimUnit' unit t) (app t unit)
+| Contraction_Unit'' :
+  forall (t : Tm)
+    (Hlc : lc t),
+    Contraction (app elimUnit'' t) t
 | Contraction_OutlPair :
-  forall v1 v2 : Tm,
-    Value v1 ->
-    Value v2 ->
+  forall (v1 v2 : Tm)
+    (Hv1 : Value v1)
+    (Hv2 : Value v2),
     Contraction (outl (pair v1 v2)) v1
 | Contraction_OutrPair :
-  forall v1 v2 : Tm,
-    Value v1 ->
-    Value v2 ->
-    Contraction (outr (pair v1 v2)) v2.
+  forall (v1 v2 : Tm)
+    (Hv1 : Value v1)
+    (Hv2 : Value v2),
+    Contraction (outr (pair v1 v2)) v2
+| Contraction_CaseInl :
+  forall (t1 t2 v : Tm)
+    (Hlc1 : lc t1)
+    (Hlc2 : lc t2)
+    (Hv : Value v),
+    Contraction (app (app (app case t1) t2) (inl v)) (app t1 v)
+| Contraction_CaseInr :
+  forall (t1 t2 v : Tm)
+    (Hlc1 : lc t1)
+    (Hlc2 : lc t2)
+    (Hv : Value v),
+    Contraction (app (app (app case t1) t2) (inr v)) (app t2 v).
 
 #[export] Hint Constructors Contraction : core.
-
-#[export] Hint Resolve lc_Value : core.
 
 Lemma lc_Contraction_l :
   forall t t' : Tm,
     Contraction t t' -> lc t.
 Proof.
-  now inversion 1; subst; eauto.
+  now inversion 1; subst; eauto 6.
 Qed.
 
 Lemma lc_Contraction_r :
   forall t t' : Tm,
     Contraction t t' -> lc t'.
 Proof.
-  inversion 1; subst; only 3-5: now eauto.
+  inversion 1; subst; try now unshelve eauto.
   - now apply lc_open'; eauto.
   - rewrite (open'_spec _ _ (fresh (l ++ fv t0))) by solve_fresh.
     apply lc_subst; [| easy].
-    apply Hcof.
+    apply Hlc.
     now solve_fresh.
 Qed.
+
+#[export] Hint Resolve lc_Contraction_l lc_Contraction_r : core.
 
 Lemma preservation_Contraction :
   forall (Γ : Ctx) (t t' : Tm) (A : Ty),
@@ -1193,18 +882,23 @@ Lemma preservation_Contraction :
     Typing Γ t' A.
 Proof.
   induction 1; inversion 1; subst.
-  - inversion H5; subst.
+  - inversion Ht1; subst.
     rewrite open'_spec with (x := fresh (l ++ fv t1)) by solve_fresh.
     apply Typing_subst with A0; [| easy].
-    apply Hcof.
+    apply Ht'.
     now solve_fresh.
   - rewrite open'_spec with (x := fresh (l0 ++ fv t)) by solve_fresh.
     apply Typing_subst with TyUnit; [| easy].
-    apply Hcof0.
+    apply Ht2.
     now solve_fresh.
   - now apply Typing_app with TyUnit.
-  - now inversion H4.
-  - now inversion H4.
+  - now inversion Ht1; subst.
+  - now inversion Ht'.
+  - now inversion Ht'.
+  - now inversion Ht1; inversion Ht2; inversion Ht0; inversion Ht4; subst;
+      inversion H15; subst; eauto.
+  - now inversion Ht1; inversion Ht2; inversion Ht0; inversion Ht4; subst;
+      inversion H15; subst; eauto.
 Qed.
 
 Inductive Abortion : Tm -> Tm -> Prop :=
@@ -1230,7 +924,21 @@ Inductive Abortion : Tm -> Tm -> Prop :=
 | Abortion_OutrPair :
   forall t : Tm,
     lc t ->
-    Abortion (outr (abort t)) (abort t).
+    Abortion (outr (abort t)) (abort t)
+| Abortion_Inl :
+  forall (t : Tm)
+    (Hlc : lc t),
+    Abortion (inl (abort t)) (abort t)
+| Abortion_Inr :
+  forall (t : Tm)
+    (Hlc : lc t),
+    Abortion (inr (abort t)) (abort t)
+| Abort_Case :
+  forall (t1 t2 t3 : Tm)
+    (Hlc1 : lc t1)
+    (Hlc2 : lc t2)
+    (Hlc3 : lc t3),
+    Abortion (app (app (app case t1) t2) (abort t3)) (abort t3).
 
 #[export] Hint Constructors Abortion : core.
 
@@ -1248,6 +956,8 @@ Proof.
   now inversion 1; subst; eauto.
 Qed.
 
+#[export] Hint Resolve lc_Abortion_l lc_Abortion_r : core.
+
 Lemma preservation_Abortion :
   forall (Γ : Ctx) (t t' : Tm) (A : Ty),
     Abortion t t' ->
@@ -1255,11 +965,14 @@ Lemma preservation_Abortion :
     Typing Γ t' A.
 Proof.
   induction 1; inversion 1; subst; constructor.
-  - now inversion H5.
-  - now inversion H4.
-  - now inversion H3.
-  - now inversion H3.
-  - now inversion H3.
+  - now inversion Ht1.
+  - now inversion Ht1.
+  - now inversion Ht1.
+  - now inversion Ht'.
+  - now inversion Ht'.
+  - now inversion Ht'.
+  - now inversion Ht'.
+  - now inversion Ht2.
 Qed.
 
 (** ** Reduction *)
@@ -1310,7 +1023,15 @@ Inductive Step : Tm -> Tm -> Prop :=
 | Step_OutrCongr :
   forall (t t' : Tm),
     Step t t' ->
-    Step (outr t) (outr t').
+    Step (outr t) (outr t')
+| Step_InlCongr :
+  forall t t' : Tm,
+    Step t t' ->
+    Step (inl t) (inl t')
+| Step_InrCongr :
+  forall t t' : Tm,
+    Step t t' ->
+    Step (inr t) (inr t').
 
 #[export] Hint Constructors Step : core.
 
@@ -1318,19 +1039,17 @@ Lemma lc_Step_l :
   forall t t' : Tm,
     Step t t' -> lc t.
 Proof.
-  induction 1; try eauto.
-  - now apply lc_Contraction_l in H.
-  - now apply lc_Abortion_l in H.
+  now induction 1; eauto.
 Qed.
 
 Lemma lc_Step_r :
   forall t t' : Tm,
     Step t t' -> lc t'.
 Proof.
-  induction 1; try eauto.
-  - now apply lc_Contraction_r in H.
-  - now apply lc_Abortion_r in H.
+  now induction 1; eauto.
 Qed.
+
+#[export] Hint Resolve lc_Step_l lc_Step_r : core.
 
 (** ** Progress and preservation *)
 
@@ -1341,9 +1060,9 @@ Lemma preservation :
     Typing Γ t2 A.
 Proof.
   intros Γ t1 t2 A Hstep; revert A.
-  induction Hstep; intros A; [| | now inversion 1; subst; econstructor; eauto..].
+  induction Hstep; intros A; [| | now inversion 1; subst; eauto..].
   - now eapply preservation_Contraction.
-  - now eapply preservation_Abortion; eauto.
+  - now eapply preservation_Abortion.
 Qed.
 
 Lemma progress :
@@ -1355,68 +1074,51 @@ Proof.
   remember [] as Γ.
   induction Ht; subst.
   - now inversion Hwf.
-  - left; constructor.
-    apply lc_abs with l.
-    intros x Hx.
-    now eapply lc_Typing, Hcof.
-  - destruct (IHHt1 eq_refl) as [ Hv | [t1' Hs1] ].
-    + inversion Hv; subst; inversion Ht1; subst.
-      * now destruct (IHHt2 eq_refl) as [ Hv2 | [t2' Hs2] ]; eauto.
-      * now apply lc_Typing in H2, Ht2; eauto.
-    + right.
-      destruct (IHHt2 eq_refl) as [ Hv2 | [t2' Hs2] ].
-      * now apply lc_Value in Hv2; eauto.
-      * now apply lc_Step_l in Hs2; eauto.
+  - now left; eauto.
+  - destruct (IHHt1 eq_refl) as [ Hv | [t1' Hs1] ]; [| now eauto].
+    inversion Hv; subst; inversion Ht1; subst; try now eauto 6.
+    + now destruct (IHHt2 eq_refl) as [ Hv2 | [t2' Hs2] ]; eauto.
+    + destruct (IHHt2 eq_refl) as [ Hv2 | [t2' Hs2] ]; [| now eauto].
+      inversion Ht0; inversion Ht4; subst.
+      inversion Ht2; subst; inversion Hv2; subst; eauto.
+      * inversion Ht2; subst; inversion Ht6.
+      * inversion Ht2; subst; inversion Ht6; subst; inversion Ht10.
   - now left.
-  - destruct (IHHt eq_refl) as [Hv | [t'' Hs] ].
-    + inversion Hv; subst; inversion Ht; subst.
-      inversion Hv; subst; inversion Ht; subst.
-      * right; exists (t2 {[ 0 ~> unit ]}).
-        constructor.
-        apply Contraction_Unit with l; intros x Hx.
-        now eapply lc_Typing, Hcof.
-      * right; exists (abort t').
-        constructor 2.
-        apply Abortion_Unit with l; [easy |].
-        intros x Hx.
-        specialize (Hcof x Hx).
-        eapply lc_Typing, Hcof.
-    + right; exists (elimUnit t'' t2).
-      apply Step_ElimUnitCongr with l ; [| easy].
-      intros x Hx.
-      now eapply lc_Typing, Hcof.
-  - destruct (IHHt1 eq_refl) as [ Hv | [t1' Hs1] ].
-    + inversion Hv; subst; inversion Ht1; subst.
-      * now apply lc_Typing in Ht2; eauto.
-      * now apply lc_Typing in H2, Ht2; eauto.
-    + right.
-      destruct (IHHt2 eq_refl) as [ Hv2 | [t2' Hs2] ].
-      * now apply lc_Value in Hv2; eauto.
-      * now apply lc_Step_l in Hs2; eauto.
-  - destruct (IHHt eq_refl) as [Hv | [t'' Hs] ].
-    + now apply lc_Value in Hv; eauto.
-    + now apply lc_Step_l in Hs; eauto.
-  - destruct (IHHt1 eq_refl) as [Hv1 | [t1' Hs1] ].
-    + now destruct (IHHt2 eq_refl) as [Hv2 | [t2' Hs1] ]; eauto.
-    + destruct (IHHt2 eq_refl) as [Hv2 | [t2' Hs2] ].
-      * now apply lc_Value in Hv2; eauto.
-      * now apply lc_Step_l in Hs2; eauto.
-  - destruct (IHHt eq_refl) as [Hv | [t'' Hs] ]; [| now eauto].
-    now inversion Hv; subst; inversion Ht; subst; eauto.
-  - destruct (IHHt eq_refl) as [Hv | [t'' Hs] ]; [| now eauto].
-    now inversion Hv; subst; inversion Ht; subst; eauto.
+  - right; destruct (IHHt eq_refl) as [Hv | [t'' Hs] ]; [| now eauto].
+    inversion Hv; subst; inversion Ht; subst; eauto 6.
+    + now inversion Ht1.
+    + now inversion Ht1.
+  - right; destruct (IHHt1 eq_refl) as [ Hv | [t1' Hs1] ]; [| now eauto].
+    inversion Hv; subst; inversion Ht1; subst; eauto.
+    + now inversion Ht1.
+    + now inversion Ht0.
+  - now left.
+  - now left; eauto.
+  - now destruct (IHHt1 eq_refl) as [| [] ], (IHHt2 eq_refl) as [| [] ]; eauto.
+  - right; destruct (IHHt eq_refl) as [Hv | [t'' Hs] ]; [| now eauto].
+    inversion Hv; subst; inversion Ht; subst; eauto.
+    + now inversion Ht1.
+    + now inversion Ht1.
+  - right; destruct (IHHt eq_refl) as [Hv | [t'' Hs] ]; [| now eauto].
+    inversion Hv; subst; inversion Ht; subst; eauto.
+    + now inversion Ht1.
+    + now inversion Ht1.
+  - now destruct (IHHt eq_refl) as [Hv | [t'' Hs] ]; eauto.
+  - now destruct (IHHt eq_refl) as [Hv | [t'' Hs] ]; eauto.
+  - now left.
 Qed.
 
 (** * Bidirectional typing *)
 
 Inductive Infer : Ctx -> Tm -> Ty -> Prop :=
 | Infer_fvar :
-  forall (Γ : Ctx) (x : Atom) (A : Ty),
-    Binds Γ x A -> Infer Γ x A
+  forall (Γ : Ctx) (x : Atom) (A : Ty)
+    (HB : Binds Γ x A),
+    Infer Γ x A
 | Infer_app  :
-  forall (Γ : Ctx) (t1 t2 : Tm) (A B : Ty),
-    Infer Γ t1 (TyFun A B) ->
-    Check Γ t2 A ->
+  forall (Γ : Ctx) (t1 t2 : Tm) (A B : Ty)
+    (Hi1 : Infer Γ t1 (TyFun A B))
+    (Hc2 : Check Γ t2 A),
     Infer Γ (app t1 t2) B
 | Infer_unit :
   forall (Γ : Ctx),
@@ -1427,42 +1129,56 @@ Inductive Infer : Ctx -> Tm -> Ty -> Prop :=
     (Hi2 : forall x : Atom, x # l -> Infer ((x, TyUnit) :: Γ) (t2 {{ 0 ~> x }}) A),
     Infer Γ (elimUnit t1 t2) A
 | Infer_pair :
-  forall (Γ : Ctx) (t1 t2 : Tm) (A B : Ty),
-    Infer Γ t1 A ->
-    Infer Γ t2 B ->
+  forall (Γ : Ctx) (t1 t2 : Tm) (A B : Ty)
+    (Hi1 : Infer Γ t1 A)
+    (Hi2 : Infer Γ t2 B),
     Infer Γ (pair t1 t2) (TyProd A B)
 | Infer_outl :
-  forall (Γ : Ctx) (t : Tm) (A B : Ty),
-    Infer Γ t (TyProd A B) ->
+  forall (Γ : Ctx) (t : Tm) (A B : Ty)
+    (Hi : Infer Γ t (TyProd A B)),
     Infer Γ (outl t) A
 | Infer_outr :
-  forall (Γ : Ctx) (t : Tm) (A B : Ty),
-    Infer Γ t (TyProd A B) ->
+  forall (Γ : Ctx) (t : Tm) (A B : Ty)
+    (Hi : Infer Γ t (TyProd A B)),
     Infer Γ (outr t) B
 
 with Check : Ctx -> Tm -> Ty -> Prop :=
 | Check_Infer :
-  forall (Γ : Ctx) (t : Tm) (A : Ty),
-    Infer Γ t A ->
+  forall (Γ : Ctx) (t : Tm) (A : Ty)
+    (Hi : Infer Γ t A),
     Check Γ t A
 | Check_abs :
   forall (Γ : Ctx) (t : Tm) (A B : Ty) (l : list Atom)
-    (Hcof : forall x : Atom, x # l -> Check ((x, A) :: Γ) (t {{0 ~> x}}) B),
+    (Hc : forall x : Atom, x # l -> Check ((x, A) :: Γ) (t {{0 ~> x}}) B),
     Check Γ (abs t) (TyFun A B)
 | Check_elimUnit' :
   forall (Γ : Ctx) (t1 t2 : Tm) (A : Ty)
     (Hc1 : Check Γ t1 TyUnit)
     (Hc2 : Check Γ t2 (TyFun TyUnit A)),
     Check Γ (elimUnit' t1 t2) A
+| Check_elimUnit'' :
+  forall (Γ : Ctx) (A : Ty),
+    Check Γ elimUnit'' (TyFun (TyFun TyUnit A) (TyFun TyUnit A))
 | Check_abort :
-  forall (Γ : Ctx) (t' : Tm) (A : Ty),
-    Check Γ t' TyEmpty ->
+  forall (Γ : Ctx) (t' : Tm) (A : Ty)
+    (Hc : Check Γ t' TyEmpty),
     Check Γ (abort t') A
 | Check_pair :
-  forall (Γ : Ctx) (t1 t2 : Tm) (A B : Ty),
-    Check Γ t1 A ->
-    Check Γ t2 B ->
-    Check Γ (pair t1 t2) (TyProd A B).
+  forall (Γ : Ctx) (t1 t2 : Tm) (A B : Ty)
+    (Hc1 : Check Γ t1 A)
+    (Hc2 : Check Γ t2 B),
+    Check Γ (pair t1 t2) (TyProd A B)
+| Check_inl :
+  forall (Γ : Ctx) (t' : Tm) (A B : Ty)
+    (Hc : Check Γ t' A),
+    Check Γ (inl t') (TySum A B)
+| Check_inr :
+  forall (Γ : Ctx) (t' : Tm) (A B : Ty)
+    (Hc : Check Γ t' B),
+    Check Γ (inr t') (TySum A B)
+| Check_case :
+  forall (Γ : Ctx) (A B C : Ty),
+    Check Γ case (TyFun (TyFun A C) (TyFun (TyFun B C) (TyFun (TySum A B) C))).
 
 #[export] Hint Constructors Infer Check : core.
 
@@ -1495,12 +1211,16 @@ Proof.
       red in Hx; rewrite in_app_iff in Hx.
       apply Typing_Check.
       * now firstorder.
-      * now apply Hcof; firstorder.
+      * now apply Hc; firstorder.
     + constructor.
       * now apply Typing_Check.
       * now apply Typing_Check.
+    + now constructor.
     + now constructor; apply Typing_Check.
     + constructor.
       * now apply Typing_Check.
       * now apply Typing_Check.
+    + now constructor; apply Typing_Check.
+    + now constructor; apply Typing_Check.
+    + now constructor.
 Qed.
